prove split/merger of owning pointers for arrays

theories/typing/array_idx.v
@@ -1,6 +1,6 @@
 From lrust.typing Require Export type.
 From lrust.typing Require Import programs
-  array int shr_bor uniq_bor product product_split.
+  array int own shr_bor uniq_bor product product_split.
 Set Default Proof Using "Type".
 
 Implicit Type 𝔄: syn_type.
@@ -8,12 +8,81 @@ Implicit Type 𝔄: syn_type.
 Section lemmas.
   Context `{!typeG Σ}.
 
+  (** * Owning Pointers *)
+
+  Fixpoint hasty_own_idxs {𝔄} (p: path) (k: nat) (ty: type 𝔄) (n: nat)
+    (i: nat) : tctx (replicate n 𝔄) :=
+    match n with 0 => +[] | S m =>
+      p +ₗ #(i * ty.(ty_size))%nat ◁ own_ptr k ty +::
+      hasty_own_idxs p k ty m (S i) end.
+
+  Lemma hasty_own_idxs_equiv {𝔄} p k (ty: _ 𝔄) n i :
+    tctx_equiv (hasty_own_idxs (p +ₗ #ty.(ty_size)) k ty n i)
+      (hasty_own_idxs p k ty n (S i)).
+  Proof.
+    apply get_tctx_equiv=> ? vπl. move: p i. induction n; [done|]=> p ?.
+    case vπl=>/= ??. f_equiv; [|done].
+    rewrite tctx_elt_interp_hasty_path; [done|]=>/=. case (eval_path p)=>//.
+    (do 2 (case=>//))=> ?. by rewrite shift_loc_assoc -Nat2Z.inj_add.
+  Qed.
+
+  Lemma tctx_split_own_array {𝔄} k (ty: _ 𝔄) n p E L :
+    tctx_incl E L +[p ◁ own_ptr k [ty; n]] (hasty_own_idxs p k ty n 0)
+      (λ post '-[al], post (vec_to_plist al)).
+  Proof.
+    move: p. elim n. { move=> ?. eapply tctx_incl_eq;
+    [by apply tctx_incl_leak_head|]=>/= ?[v[]]. by inv_vec v. } move=>/= ? IH ?.
+    eapply tctx_incl_eq. { eapply tctx_incl_trans; [by eapply subtype_tctx_incl;
+    eapply own_subtype, proj1, array_succ_prod|]. eapply tctx_incl_trans;
+    [by eapply tctx_split_own_prod|]. apply (tctx_incl_app +[_] +[_]);
+    [by apply tctx_to_shift_loc_0, _|]. eapply tctx_incl_trans; [by apply IH|].
+    eapply proj1, hasty_own_idxs_equiv. } move=>/= ?[v[]]. by inv_vec v.
+  Qed.
+
+  Lemma tctx_extract_split_own_array {𝔄 𝔄' 𝔅l ℭl} (t: _ 𝔄) k (ty: _ 𝔄') n
+    (T: _ 𝔅l) (T': _ ℭl) tr p E L :
+    tctx_extract_elt E L t (hasty_own_idxs p k ty n 0) T' tr →
+    tctx_extract_elt E L t (p ◁ own_ptr k [ty; n] +:: T) (T' h++ T) (λ post
+      '(al -:: bl), tr (λ '(a -:: cl), post (a -:: cl -++ bl)) (vec_to_plist al)).
+  Proof.
+    move=> ?. eapply tctx_incl_eq. { eapply (tctx_incl_frame_r +[_] (_ +:: _)).
+    eapply tctx_incl_trans; by [apply tctx_split_own_array|]. }
+    move=>/= ?[??]. rewrite /trans_upper /=. f_equal. fun_ext. by case.
+  Qed.
+
+  Lemma tctx_merge_own_array {𝔄} k (ty: _ 𝔄) n p E L :
+    tctx_incl E L (hasty_own_idxs p k ty (S n) 0) +[p ◁ own_ptr k [ty; S n]]
+      (λ post al, post -[plist_to_vec al]).
+  Proof.
+    move: p. elim: n. { move=> ?. eapply tctx_incl_eq. { eapply tctx_incl_trans;
+    [by apply tctx_of_shift_loc_0|]. eapply subtype_tctx_incl, own_subtype, proj2,
+    array_one. } by move=> ?[?[]]. } move=>/= ? IH ?. eapply tctx_incl_eq. {
+    eapply tctx_incl_trans; [|by eapply subtype_tctx_incl, own_subtype, proj2,
+    array_succ_prod]. eapply tctx_incl_trans; [|by eapply tctx_merge_own_prod].
+    apply (tctx_incl_app +[_] +[_]); [by apply tctx_of_shift_loc_0|].
+    eapply tctx_incl_trans; [|by apply IH]. apply (tctx_incl_app +[_] +[_]);
+    [|by eapply proj2, hasty_own_idxs_equiv]. rewrite Nat2Z.inj_add.
+    eapply proj2, tctx_shift_loc_assoc. } by move=>/= ?[?[??]].
+  Qed.
+
+  Lemma tctx_extract_merge_own_array {𝔄 𝔅l ℭl} k (ty: _ 𝔄) n
+    (T: _ 𝔅l) (T': _ ℭl) tr p E L :
+    tctx_extract_ctx E L (hasty_own_idxs p k ty (S n) 0) T T' tr →
+    tctx_extract_elt E L (p ◁ own_ptr k [ty; S n]) T T' (λ post, tr
+      (λ acl, let '(al, cl) := psep acl in post (plist_to_vec al -:: cl))).
+  Proof.
+    move=> ?. eapply tctx_incl_eq. { eapply tctx_incl_trans; [done|].
+    apply (tctx_incl_frame_r _ +[_]), tctx_merge_own_array. } done.
+  Qed.
+
+  (** * Shared References *)
+
   Lemma tctx_idx_shr_array {𝔄 𝔅l} (ty: _ 𝔄) n κ p (i: fin n) (T: _ 𝔅l) E L :
     tctx_incl E L (p ◁ &shr{κ} [ty; n] +:: T)
       (p +ₗ #(i * ty.(ty_size))%nat ◁ &shr{κ} ty +:: T)
       (λ post '(xl -:: bl), post (xl !!! i -:: bl))%type.
   Proof.
-    iIntros (??[??]?) "_ _ _ _ $ [p T] Obs !>". iExists (_ -:: _).
+    iIntros (??[??]?) "_ _ _ _ $ [p T] Obs !>". iExists (_-::_).
     iFrame "Obs T". iDestruct "p" as ([[]|][|]Ev) "[⧖ ?]"=>//=. iExists _, _.
     iSplit; [by rewrite/= Ev|]. iFrame "⧖". by rewrite big_sepL_vlookup vfunsep_lookup.
   Qed.
@@ -55,6 +124,8 @@ Section lemmas.
     f_equal. fun_ext. by case=> [?[??]].
   Qed.
 
+  (** * Unique References *)
+
   Fixpoint hasty_uniq_idxs {𝔄} (p: path) (κ: lft) (ty: type 𝔄) (n: nat)
     (i: nat) : tctx (replicate n (𝔄 * 𝔄)%ST) :=
     match n with 0 => +[] | S m =>
@@ -64,16 +135,15 @@ Section lemmas.
   Lemma tctx_split_uniq_array {𝔄} (ty: _ 𝔄) n κ p E L :
     lctx_lft_alive E L κ →
     tctx_incl E L +[p ◁ &uniq{κ} [ty; n]] (hasty_uniq_idxs p κ ty n 0)
-      (λ post '-[(al, al')], post
-        (vec_to_plist (vzip al al': vec (𝔄 * 𝔄)%ST _))).
+      (λ post '-[(al, al')], post (vec_to_plist (vzip al al'))).
   Proof.
     move=> ?. move: p. elim: n. { move=> ?. eapply tctx_incl_eq;
-    [apply tctx_incl_leak_head|]=>/= ?[[v v'][]]. inv_vec v. by inv_vec v'. }
+    [by apply tctx_incl_leak_head|]=>/= ?[[v v'][]]. inv_vec v. by inv_vec v'. }
     move=>/= n IH p. eapply tctx_incl_eq. { eapply tctx_incl_trans;
     [eapply tctx_uniq_eqtype; by [apply array_succ_prod|apply _|]|].
-    eapply tctx_incl_trans. { eapply (tctx_incl_frame_r +[_]).
-    by eapply tctx_split_uniq_prod. } apply (tctx_incl_app +[_] +[_]);
-    [apply tctx_to_shift_loc_0, _|]. eapply tctx_incl_trans; [apply IH|].
+    eapply tctx_incl_trans; [by eapply (tctx_incl_frame_r +[_]),
+    tctx_split_uniq_prod|]. apply (tctx_incl_app +[_] +[_]);
+    [by apply tctx_to_shift_loc_0, _|]. eapply tctx_incl_trans; [apply IH|].
     eapply proj1, get_tctx_equiv=> ? vπl. move: p 0. clear.
     induction n; [done|]=> p ?. case vπl=>/= ??. f_equiv; [|done].
     rewrite tctx_elt_interp_hasty_path; [done|]=>/=. case (eval_path p)=>//.
@@ -96,5 +166,6 @@ Section lemmas.
 
 End lemmas.
 
-Global Hint Resolve tctx_extract_idx_shr_array tctx_extract_split_uniq_array
-  | 5 : lrust_typing.
+Global Hint Resolve tctx_extract_split_own_array
+  tctx_extract_idx_shr_array tctx_extract_split_uniq_array | 5 : lrust_typing.
+Global Hint Resolve tctx_extract_merge_own_array | 40 : lrust_typing_merge.
